% !TEX program = latex

\documentclass[12pt]{article}

\usepackage[right=1in]{geometry}

\usepackage{mathtools}
\usepackage{cancel}
\usepackage{xfrac}

\usepackage{fancyhdr}

\pagestyle{fancy}
\fancyhead[L]{Training Exercise 1.2}
\fancyhead[R]{MOOC Econometrics}

\begin{document}

\section*{Question 1}
Show that in the regression model $log(y_i) = \alpha + \beta\ log(x_i) + \epsilon_i$ , the elasticity of $y$ with respect to $x$ is equal to $\beta$ (that is, does not depend on the values of $x_i$ and $y_i$).

\subsection*{Answer}

According to the definition of the elasticity, (noted in lecture slides)
\[
    \text{Elasticity} = \frac{\sfrac{dy}{y}}{\sfrac{dx}{x}} = \frac{dy}{dx} \times \frac{x}{y}
\]

By exponentiating both sides of the model
\begin{align*}
    y_i &= e^{(\alpha + \epsilon_i)} \times e^{(\beta \times log(x_i))}\\
        &= e^{(\alpha + \epsilon_i)} \times x_i^\beta\\
\end{align*}

Now we can calculate the derivative of $y$ with respect to $x$
\[
    \frac{d y_i}{d x_i} = e^{\alpha + \epsilon_i} \times \beta \times x_i^{\beta - 1} = \beta \times \frac{y_i}{x_i}
\]

By substituting the derivative of $y$ with respect to $x$ into the elasticity equation
\[
    \text{Elasticity} = \frac{dy}{dx} \times \frac{x}{y} = \beta\ \frac{\cancel{y}}{\cancel{x}} \times \frac{\cancel{x}}{\cancel{y}} = \beta
\]

\newpage
\section*{Question 2}
Determine the elasticity of $y$ with respect to $x$ in the model $y_i = \alpha + \beta\ log(x_i) + \epsilon_i$.

\subsection*{Answer}
The process is the same as in the previous question.

First we calculate the derivative of $y$ with respect to $x$
\[
    \frac{d y_i}{d x_i} = \beta \times \frac{1}{x_i}
\]

Now the elasticity is
\[
    \text{Elasticity} = \frac{dy}{dx} \times \frac{x}{y} = \beta \times \frac{\cancel{x}}{y} \times \frac{1}{\cancel{x}} = \beta \times \frac{1}{y}
\]

\section*{Question 3}
Determine the elasticity of $y$ with respect to $x$ in the model $log(y_i) = \alpha + \beta\ x_i + \epsilon_i$.

\subsection*{Answer}
Exponentiate the model
\[
    y_i = e^{(\alpha + \epsilon_i)} \times e^{(\beta x_i)}\\
\]

By taking the derivative of $y$ with respect to $x$
\[
    \frac{d y_i}{d x_i} = e^{\alpha + \epsilon_i} \times \beta \times e^{(\beta x_i)} = \beta \times y_i
\]

Elasticity would be
\[
    \text{Elasticity} = \frac{dy}{dx} \times \frac{x}{y} = \beta \times y \times \frac{x}{y} = \beta \times x_i
\]

\end{document}